coq/lib/P4flat/P4flatToGCL.v
@@ -6,57 +6,52 @@ Require Import Poulet4.P4flat.GGCL.
 Require Import Poulet4.Monads.Option.
 Require Import Poulet4.Monads.ExceptionState.
 Require Import Poulet4.Utils.Envn.
+Require Import Poulet4.Utils.AList.
 Require Poulet4.Utils.NameGen.
+Require stdpp.list.
 Require stdpp.gmap.
 Print gmap.gmap.
 Import ResultNotations.
-Import Dijkstra.
 
 Module GEN := NameGen.NameGenParam.
 Open Scope string_scope.
 
-Definition var := string.
+  (* A map from de Bruijn indices to fresh names. *)
+  Definition idx_map := list string.
+  Definition idx_map_init : idx_map := [].
+  Inductive vartyp :=
+  | LocalVar (typ: AST.Typ.t)
+  | TableFun (key_typ: list Typ.t) (act_arg_typs: list Typ.t).
+  Definition var_env := GEN.t vartyp.
+  Definition var_env_init : var_env := GEN.init.
 
-Record tbl_sig :=
-  { tbl_sig_key: AST.Typ.t;
-    tbl_sig_acts: list (string * Exp.args * Stm.t) }.
+  Notation M := (state_monad var_env string).
 
-(* A map from table names to table signatures. *)
-Definition tbl_map :=
-  Env.t string tbl_sig.
+  Definition freshen_name (s: string) (t: AST.Typ.t) : M string :=
+    let* e := get_state in
+    let (s, e') := GEN.freshen e s (LocalVar t) in
+    put_state e';;
+    mret s.
 
-(* A map from de Bruijn indices to fresh names. *)
-Definition idx_map := list string.
-Definition idx_map_init : idx_map := [].
-Definition var_env := GEN.t AST.Typ.t.
-Definition var_env_init : var_env := GEN.init.
+  Definition declare_var (name: string) (typ: AST.Typ.t) (m: idx_map) : M idx_map :=
+    let* name' := freshen_name name typ in
+    mret (name' :: m).
 
-Notation M := (state_monad var_env string).
+  Definition declare_param (name: string) (param: CUB.Typ.param) : idx_map -> M idx_map :=
+    let typ := match param with
+               | PAIn t
+               | PAOut t 
+               | PAInOut t => t
+               end
+    in
+    declare_var name typ.
+  
+  Definition declare_params (params: CUB.Typ.params) : idx_map -> M idx_map :=
+    fold_left_monad (fun m '(name, p) => declare_param name p m) params.
 
-Definition freshen_name (s: string) (t: AST.Typ.t) : M string :=
-  let* e := get_state in
-  let (s, e') := GEN.freshen e s t in
-  put_state e';;
-  mret s.
+  Definition find_var (m: idx_map) (k: nat) : M string :=
+    from_opt (nth_error m k) "find_var: index not found in idx_map".
 
-Definition declare_var (name: string) (typ: AST.Typ.t) (m: idx_map) : M idx_map :=
-  let* name' := freshen_name name typ in
-  mret (name' :: m).
-
-Definition declare_param (name: string) (param: CUB.Typ.param) : idx_map -> M idx_map :=
-  let typ := match param with
-             | PAIn t
-             | PAOut t 
-             | PAInOut t => t
-             end
-  in
-  declare_var name typ.
-    
-Definition declare_params (params: CUB.Typ.params) : idx_map -> M idx_map :=
-  fold_left_monad (fun m '(name, p) => declare_param name p m) params.
-
-Definition find_var (m: idx_map) (k: nat) : M string :=
-  from_opt (nth_error m k) "find_var: index not found in idx_map".
 
 Inductive p4sorts :=
 | Bool
@@ -68,20 +63,27 @@ Scheme Equality for p4sorts.
 Instance p4sorts_EqDec : EqDec p4sorts eq := 
   p4sorts_eq_dec.
 
-Inductive p4funs :=
+(* Function symbols common to all P4 programs. *)
+Inductive p4funs_base :=
 | BTrue
 | BFalse
 | BBitLit (width: N) (val: Z)
-| BTable (name: string)
 | BProj1
-| BProj2
-(* Better for this to be an enum or at least an integer *)
-| BAction (name: string)
-| BVar (name: string).
-Scheme Equality for p4funs.
+| BProj2.
 #[global]
-Instance p4funs_EqDec : EqDec p4funs eq := 
-  p4funs_eq_dec.
+Instance p4funs_base_EqDec : EqDec p4funs_base eq.
+Admitted.
+
+(* Function symbols arising from particular programs. *)
+Inductive p4funs_prog :=
+| BTable (name: string)
+| BAction (name: string).
+#[global]
+Instance p4funs_prog_EqDec : EqDec p4funs_prog eq.
+Admitted.
+
+Definition p4funs : Type :=
+  p4funs_base + p4funs_prog.
 
 Inductive p4rels :=
 (* no relation symbols *)
@@ -98,35 +100,36 @@ Definition initial_p4sig : p4sig :=
   {| Sig.sig_sorts :=
     fun s =>
       match s with
-      | Bool => Some 0
-      | ActionName => Some 0
-      | _ => None
+      | Bool => true
+      | ActionName => true
+      | Bit k => true
+      | _ => false
       end;
     Sig.sig_funs := fun f =>
-                        if f == Sig.SSimple BTrue
-                        then Some ([], (Sig.SSimple Bool))
-                        else if f == Sig.SSimple BFalse
-                             then Some ([], (Sig.SSimple Bool))
-                             else None;
-     Sig.sig_rels := fun _ => None |}.
+                      if Sig.ident_EqDec f (Sig.SSimple (inl BTrue))
+                      then Some ([], (Sig.SSimple Bool))
+                      else if f == Sig.SSimple (inl BFalse)
+                           then Some ([], (Sig.SSimple Bool))
+                           else None;
+    Sig.sig_rels := fun _ => None |}.
+  
+Definition mk_action (name: string) : Spec.tm string p4funs :=
+  Spec.TFun (Sig.SSimple (inr (BAction name))) [].
 
-Definition mk_action (name: string) : Spec.tm var p4funs :=
-  Spec.TFun (Sig.SSimple (BAction name)) [].
-
-Definition lhs_to_var (m: idx_map) (e: Exp.t) : M var :=
+Definition lhs_to_var (m: idx_map) (e: Exp.t) : M string :=
   match e with
   | Exp.Var _ _ idx => find_var m idx
   | _ => error "lvals other than vars are not yet implemented"
   end.
 
-Definition e_to_tm (e: Exp.t) : M (Spec.tm var p4funs) :=
+Definition e_to_tm (e: Exp.t) : M (Spec.tm string p4funs) :=
   match e with
-  | Exp.Bit width val => mret (Spec.TFun (Sig.SSimple (BBitLit width val)) [])
+  | Exp.Bit width val => mret (Spec.TFun (Sig.SSimple (inl (BBitLit width val))) [])
   | Exp.Var _ name _ => mret (Spec.TVar name)
   | _ => error "e_to_tm unimplemented"
   end.
 
-Fixpoint s_to_stmt (m: idx_map) (s: Stm.t) : M (stmt var p4funs p4rels) :=
+Fixpoint s_to_stmt (m: idx_map) (s: Stm.t) : M (stmt string p4funs p4rels) :=
   match s with
   | Stm.Skip => mret (GSkip _ _ _)
   | Stm.Ret e => (error "return unimplemented")
@@ -141,9 +144,9 @@ Fixpoint s_to_stmt (m: idx_map) (s: Stm.t) : M (stmt var p4funs p4rels) :=
       let* key' := sequence (List.map e_to_tm key) in
       (* XXX generate an actually fresh variable here *)
       let result_var := ctrl_plane_name ++ "__res" in
-      let call_tm := Spec.TFun (Sig.SSimple (BTable ctrl_plane_name)) key' in
+      let call_tm := Spec.TFun (Sig.SSimple (inr (BTable ctrl_plane_name))) key' in
       let call_stmt := GAssign result_var call_tm in
-      let act_choice := Spec.TFun (Sig.SSimple BProj1) [Spec.TVar result_var] in
+      let act_choice := Spec.TFun (Sig.SSimple (inl BProj1)) [Spec.TVar result_var] in
       let* actions_stmts :=
         sequence (List.map (fun '(name, params, stmt) =>
                               let* stmt' := s_to_stmt m stmt in  
@@ -166,12 +169,12 @@ Fixpoint s_to_stmt (m: idx_map) (s: Stm.t) : M (stmt var p4funs p4rels) :=
       mret (GSeq head' tail')
   | Stm.Cond guard tru_blk fls_blk =>
       let* guard' := (e_to_tm guard) in
-      let then_cond := Spec.FEq guard' (Spec.TFun (Sig.SSimple BTrue) []) in
+      let then_cond := Spec.FEq guard' (Spec.TFun (Sig.SSimple (inl BTrue)) []) in
       let else_cond := Spec.FNeg then_cond in
       let* tru_blk' := s_to_stmt m tru_blk in
       let* fls_blk' := s_to_stmt m fls_blk in
       mret (GChoice (GSeq (GAssume then_cond) tru_blk')
-                       (GSeq (GAssume else_cond) fls_blk'))
+                    (GSeq (GAssume else_cond) fls_blk'))
   | Stm.SetValidity _ _ =>
       (error "SetValidity unimplemented")
   end.
@@ -188,31 +191,57 @@ Definition typ_to_sort (t: Typ.t) : option p4sorts :=
   | Typ.Var k => None
   end.
 
-Definition typed_var_to_ranked_sym (typed_var: string * Typ.t) : option (p4funs * (Sig.rank p4sorts * Sig.sort p4sorts)) :=
-  let (var, type) := typed_var in
-  let* ret := typ_to_sort type in
-  mret (BVar var, ([], Sig.SSimple ret)).
+Definition nonempty_list_to_prod (l: list p4sorts) : option p4sorts :=
+  match l with
+  | x :: l' =>
+      Some (List.fold_left Prod l' x)
+  | [] =>
+      None
+  end.
 
-Definition var_env_to_fsig (env: var_env) : option (Sig.fsignature p4sorts p4funs p4rels) :=
-  let bindings : list (string * Typ.t) := gmap.gmap_to_list env in
-  let* funs := sequence (map typed_var_to_ranked_sym bindings) in
-  mret {| Sig.fsig_sorts := [];
-          Sig.fsig_funs := funs;
-          Sig.fsig_rels := [] |}.
+Definition vartyp_to_var_or_sym (typed_var: string * vartyp)
+  : option (string * Sig.sort p4sorts + p4funs_prog * (Sig.rank p4sorts * Sig.sort p4sorts)) :=
+  let (var, vt) := typed_var in
+  match vt with
+  | LocalVar type =>
+      let* sort := typ_to_sort type in
+      mret (inl (var, Sig.SSimple sort))
+  | TableFun key_typs act_arg_typs =>
+      let* args := sequence (List.map typ_to_sort key_typs) in
+      let* rets := sequence (List.map typ_to_sort act_arg_typs) in
+      let* ret := nonempty_list_to_prod rets in
+      mret (inr (BTable var, (List.map Sig.SSimple args, Sig.SSimple ret)))
+  end.
 
-Definition prog_to_sig_stmt (p: Top.prog) : M (Sig.fsignature p4sorts p4funs p4rels *
-                                               stmt var p4funs p4rels) :=
+Definition vartyps_to_vars_syms
+           (bindings: list (string * vartyp))
+  : option (list (string * Sig.sort p4sorts) *
+           (list (p4funs_prog * (Sig.rank p4sorts * Sig.sort p4sorts)))) :=
+  let* vars_or_syms := sequence (map vartyp_to_var_or_sym bindings) in
+  Some (base.omap option.maybe_inl vars_or_syms,
+        base.omap option.maybe_inr vars_or_syms).
+
+Definition var_env_to_vars_funs (env: var_env) : option (AList string (Sig.sort p4sorts) eq *
+                                                         AList p4funs_prog (Sig.rank p4sorts * Sig.sort p4sorts) eq) :=
+  let bindings : list (string * vartyp) := gmap.gmap_to_list env in
+  vartyps_to_vars_syms bindings.
+
+Definition prog_to_sig_stmt (p: Top.prog)
+  : M (AList p4funs_prog (Sig.rank p4sorts * Sig.sort p4sorts) eq *
+       list (string * Sig.sort p4sorts) *
+       stmt string p4funs p4rels) :=
   let* (_, main_args) := from_result (Top.find_decl "main" p
-                                      >>= Top.expect_pkg) in
+                                                    >>= Top.expect_pkg) in
   let* ctrl := match main_args with
                | [ctrl] => mret ctrl
                | _ => error "wrong number of args to main pkg (expected exactly 1)"
                end in
   let* (_, eparams, params, cstmt) := from_result (Top.find_decl ctrl p
-                                                   >>= Top.expect_controlblock) in
+                                                                 >>= Top.expect_controlblock) in
   let* m := declare_params params idx_map_init in 
   let* res := s_to_stmt m cstmt in
   let* env := get_state in
-  let* fsig := ExceptionState.from_opt (var_env_to_fsig env)
-                                       "conversion to fsig failed" in
-  mret (fsig, res).
+  let* (vars, fsig) :=
+    ExceptionState.from_opt (var_env_to_vars_funs env)
+                            "conversion to fsig failed" in
+  mret (fsig, vars, res).
