coq/lib/P4flat/GGCL.v
@@ -3,86 +3,110 @@ Require Import Coq.Classes.EquivDec.
 Require Import Poulet4.P4flat.Sig.
 Require Import Poulet4.P4flat.Spec.
 Require Import Poulet4.Monads.Result.
+Require Import Poulet4.Utils.AList.
 Import ResultNotations.
+Open Scope list_scope.
 
-Module Dijkstra.
-  Section Dijkstra.
-    Variable (var: Type).
-    Context `{Equivalence var eq}.
-    Context `{EqDec var eq}.
-    Variables (sort_sym fun_sym rel_sym: vocab).
-    Context `{@EqDec fun_sym eq eq_equivalence}.
-    Context `{@EqDec rel_sym eq eq_equivalence}.
-    Context `{@EqDec sort_sym eq eq_equivalence}.
-    Variable (sig: signature sort_sym fun_sym rel_sym).
+Section GGCL.
+  Variable (var: Type).
+  Context `{Equivalence var eq}.
+  Context `{EqDec var eq}.
+  Variables (sort_sym fun_sym rel_sym: vocab).
+  Context `{@EqDec fun_sym eq eq_equivalence}.
+  Context `{@EqDec rel_sym eq eq_equivalence}.
+  Context `{@EqDec sort_sym eq eq_equivalence}.
+  Variable (sig: signature sort_sym fun_sym rel_sym).
 
-    Inductive stmt : Type :=
-    | GSkip
-    | GAssign (lhs : var)
-              (rhs : Spec.tm var fun_sym)
-    | GSeq (g1 g2 : stmt)
-    | GChoice (g1 g2 : stmt)
-    | GAssume (phi : Spec.fm var fun_sym rel_sym)
-    | GAssert (phi : Spec.fm var fun_sym rel_sym).
+  Inductive stmt : Type :=
+  | GSkip
+  | GAssign (lhs : var)
+            (rhs : Spec.tm var fun_sym)
+  | GSeq (g1 g2 : stmt)
+  | GChoice (g1 g2 : stmt)
+  | GAssume (phi : Spec.fm var fun_sym rel_sym)
+  | GAssert (phi : Spec.fm var fun_sym rel_sym).
 
-    (* Naive WP. *)
-    Fixpoint wp (s: stmt) (phi: Spec.fm var fun_sym rel_sym)
-      : Spec.fm var fun_sym rel_sym :=
-      match s with
-      | GSkip => phi
-      | GAssign lhs rhs => Spec.fm_subst lhs rhs phi
-      | GSeq g1 g2 => wp g1 (wp g2 phi)
-      | GChoice g1 g2 => FOr (wp g1 phi) (wp g2 phi)
-      | GAssume psi => FImpl psi phi
-      | GAssert psi => FAnd psi phi
-      end.
-
-  End Dijkstra.
-  Arguments GAssign {var fun_sym rel_sym}.
-  Arguments GSeq    {var fun_sym rel_sym}.
-  Arguments GChoice {var fun_sym rel_sym}.
-  Arguments GAssume {var fun_sym rel_sym}.
-  Arguments GAssert {var fun_sym rel_sym}.
-
-  Fixpoint stmt_map_vars {V W fun_sym rel_sym} (m: V -> W) (s: stmt V fun_sym rel_sym)
-    : stmt W fun_sym rel_sym :=
+  (* Naive WP. *)
+  Fixpoint wp (s: stmt) (phi: Spec.fm var fun_sym rel_sym)
+    : Spec.fm var fun_sym rel_sym :=
     match s with
-    | GSkip _ _ _ => GSkip _ _ _
-    | GAssign lhs rhs => GAssign (m lhs) (Spec.tm_map_vars m rhs)
-    | GSeq g1 g2 => GSeq (stmt_map_vars m g1) (stmt_map_vars m g2) 
-    | GChoice g1 g2 => GChoice (stmt_map_vars m g1) (stmt_map_vars m g2)
-    | GAssume phi => GAssume (Spec.fm_map_vars m phi)
-    | GAssert phi => GAssert (Spec.fm_map_vars m phi)
+    | GSkip => phi
+    | GAssign lhs rhs => Spec.fm_subst lhs rhs phi
+    | GSeq g1 g2 => wp g1 (wp g2 phi)
+    | GChoice g1 g2 => FOr (wp g1 phi) (wp g2 phi)
+    | GAssume psi => FImpl psi phi
+    | GAssert psi => FAnd psi phi
     end.
 
-  Section Products.
-    Context {V1: Type}.
-    Context `{Equivalence V1 eq}.
-    Context `{EqDec V1 eq}.
-    Context {V2: Type}.
-    Context `{Equivalence V2 eq}.
-    Context `{EqDec V2 eq}.
-    Variables (sort_sym fun_sym rel_sym: vocab).
-    Context `{@EqDec fun_sym eq eq_equivalence}.
-    Context `{@EqDec rel_sym eq eq_equivalence}.
-    Context `{@EqDec sort_sym eq eq_equivalence}.
-    Variable (sig: signature sort_sym fun_sym rel_sym).
+End GGCL.
+Arguments GAssign {var fun_sym rel_sym}.
+Arguments GSeq    {var fun_sym rel_sym}.
+Arguments GChoice {var fun_sym rel_sym}.
+Arguments GAssume {var fun_sym rel_sym}.
+Arguments GAssert {var fun_sym rel_sym}.
 
-    (* Note this requires the two programs already agree on a signature
-       [sig], but you will want them to at least have disjoint table
-       signatures when dealing with table programs. *)
-    Definition seq_prod_prog
-               (s1: stmt V1 fun_sym rel_sym)
-               (s2: stmt V2 fun_sym rel_sym)
-      : stmt (V1 + V2) fun_sym rel_sym :=
-      (* <s1|; |s2> *)
-      GSeq (stmt_map_vars inl s1) (stmt_map_vars inr s2).
+Fixpoint stmt_map_vars {V W fun_sym rel_sym} (m: V -> W) (s: stmt V fun_sym rel_sym)
+  : stmt W fun_sym rel_sym :=
+  match s with
+  | GSkip _ _ _ => GSkip _ _ _
+  | GAssign lhs rhs => GAssign (m lhs) (Spec.tm_map_vars m rhs)
+  | GSeq g1 g2 => GSeq (stmt_map_vars m g1) (stmt_map_vars m g2) 
+  | GChoice g1 g2 => GChoice (stmt_map_vars m g1) (stmt_map_vars m g2)
+  | GAssume phi => GAssume (Spec.fm_map_vars m phi)
+  | GAssert phi => GAssert (Spec.fm_map_vars m phi)
+  end.
 
-    Definition seq_prod_wp
-               (s1: stmt V1 fun_sym rel_sym)
-               (s2: stmt V2 fun_sym rel_sym)
-               spec :=
-      wp _ _ _ (seq_prod_prog s1 s2) spec.
+Fixpoint stmt_map_funs {V F G rel_sym} (m: F -> G) (s: stmt V F rel_sym)
+  : stmt V G rel_sym :=
+  match s with
+  | GSkip _ _ _ => GSkip _ _ _
+  | GAssign lhs rhs => GAssign lhs (Spec.tm_map_funs m rhs)
+  | GSeq g1 g2 => GSeq (stmt_map_funs m g1) (stmt_map_funs m g2) 
+  | GChoice g1 g2 => GChoice (stmt_map_funs m g1) (stmt_map_funs m g2)
+  | GAssume phi => GAssume (Spec.fm_map_funs m phi)
+  | GAssert phi => GAssert (Spec.fm_map_funs m phi)
+  end.
 
-  End Products.
-End Dijkstra.
+Section Products.
+  Context {V1: Type}.
+  Context `{Equivalence V1 eq}.
+  Context `{EqDec V1 eq}.
+  Context {V2: Type}.
+  Context `{Equivalence V2 eq}.
+  Context `{EqDec V2 eq}.
+  Variables (sort_sym fun_sym F1 F2 rel_sym: vocab).
+  Context `{@EqDec fun_sym eq eq_equivalence}.
+  Context `{@EqDec rel_sym eq eq_equivalence}.
+  Context `{@EqDec sort_sym eq eq_equivalence}.
+  Variable (sig: signature sort_sym fun_sym rel_sym).
+
+  Definition alist_sum {A B V} (l1: AList A V eq) (l2: AList B V eq) : AList (A + B) V eq :=
+    List.map (fun '(k, v) => (inl k, v)) l1 ++
+    List.map (fun '(k, v) => (inr k, v)) l2.
+
+  Definition fix_fun1 (f: fun_sym + F1) : fun_sym + (F1 + F2) := 
+    FunUtil.map_sum id inl f.
+
+  Definition fix_fun2 (f: fun_sym + F2) : fun_sym + (F1 + F2) := 
+    FunUtil.map_sum id inr f.
+
+  (* Note this requires the two programs already agree on a signature
+     [sig], but you will want them to at least have disjoint table
+     signatures when dealing with table programs. *)
+  Definition seq_prod_prog
+             (fsig1: AList F1 (rank sort_sym * sort sort_sym) eq)
+             (gamma1: list (V1 * sort sort_sym))
+             (s1: stmt V1 (fun_sym + F1)%type rel_sym)
+             (fsig2: AList F2 (rank sort_sym * sort sort_sym) eq)
+             (gamma2: AList V2 (sort sort_sym) eq)
+             (s2: stmt V2 (fun_sym + F2)%type rel_sym)
+    : AList (F1 + F2)%type (rank sort_sym * sort sort_sym) eq *
+      AList (V1 + V2)%type (sort sort_sym) eq *
+      stmt (V1 + V2) (fun_sym + (F1 + F2))%type rel_sym :=
+    (* <s1|; |s2> *)
+    (alist_sum fsig1 fsig2,
+     alist_sum gamma1 gamma2,
+     GSeq (stmt_map_funs fix_fun1 (stmt_map_vars inl s1))
+          (stmt_map_funs fix_fun2 (stmt_map_vars inr s2))).
+
+End Products.
